Continue with proof

PolyMu_Bisim_Invariance.thy
@@ -261,42 +261,106 @@ definition R_closed :: "(('\<iota> \<Rightarrow> 's) set) \<Rightarrow> bool" wh
 definition env_R_closed :: "('\<iota>,'s,'var) env \<Rightarrow> bool" where
   "env_R_closed \<rho> \<longleftrightarrow> (\<forall>X. R_closed (\<rho> X))"
 
+(* little helpers *)
 lemma perm: "(s,t)\<in>R \<Longrightarrow> (perm_tup \<pi> s, perm_tup \<pi> t)\<in>R"
   by (simp add: perm_closed)
 
+lemma pos_Dia_inv: "pos X (Dia i a \<phi>) \<Longrightarrow> pos X \<phi>"
+  by (auto elim: pos.cases)
+
+lemma pos_Perm_inv: "pos X (Perm \<pi> \<phi>) \<Longrightarrow> pos X \<phi>"
+  by (auto elim: pos.cases)
+
+lemma pos_NotE: "pos X (Not \<phi>) \<Longrightarrow> False"
+  using pos.cases by fastforce
+
+lemma pos_And_inv1: "pos X (And \<phi> \<psi>) \<Longrightarrow> pos X \<phi>"
+  using pos.cases by fastforce
+
+lemma pos_And_inv2: "pos X (And \<phi> \<psi>) \<Longrightarrow> pos X \<psi>"
+  using pos.cases by fastforce
+
+definition lift_set :: "(('\<iota>,'s) tup) set \<Rightarrow> (('\<iota>,'t) tup) set"
+  where "lift_set S = { v. \<exists>u\<in>S. (u,v) \<in> R }"
+
+lemma lift_env_update:
+  "lift_env (\<rho>(X := S)) = (lift_env \<rho>)(X := lift_set S)"
+  by (auto simp: lift_env_def lift_set_def fun_eq_iff split: if_splits)
+
+primrec funpow  where
+  "funpow 0 f x = x"
+| "funpow (Suc n) f x = f (funpow n f x)"
+
+definition appr
+  where "appr F n = funpow n F {}"
+
+definition appr'
+  where "appr' G n = funpow n G {}"
+
+lemma appr_0[simp]: "appr F 0 = {}"
+  by (simp add: appr_def)
+
+lemma appr_Suc[simp]: "appr F (Suc n) = F (appr F n)"
+  by (simp add: appr_def funpow_Suc_right)
+
+lemma appr'_0[simp]: "appr' G 0 = {}"
+  by (simp add: appr'_def)
+
+lemma appr'_Suc[simp]: "appr' G (Suc n) = G (appr' G n)"
+  by (simp add: appr'_def funpow_Suc_right)
+
+(* increasing chain *)
+lemma appr_chain: 
+  assumes "mono F" 
+  shows "appr F n \<subseteq> appr F (Suc n)"
+proof (induction n)
+  case 0
+  show ?case by simp
+next
+  case (Suc n)
+  from assms Suc.IH have "F (appr F n) \<subseteq> F (appr F (Suc n))"
+    by (rule monoD)
+  then show ?case by simp
+qed
+
+lemma appr'_chain: 
+  assumes "mono G" 
+  shows "appr' G n \<subseteq> appr' G (Suc n)"
+proof (induction n)
+  case 0
+  show ?case by simp
+next
+  case (Suc n)
+  from assms Suc.IH have "G (appr' G n) \<subseteq> G (appr' G (Suc n))"
+    by (rule monoD)
+  then show ?case by simp
+qed
+
+(* preservation lemma *)
 lemma preservation:
-  assumes "(s,t)\<in>R" and "env_R_closed \<rho>"
+  assumes "(s,t)\<in>R" and "env_R_closed \<rho>" and "pos X \<phi>"
   shows "(s \<in> eval M \<rho> \<phi>) \<longleftrightarrow> (t \<in> eval N (lift_env \<rho>) \<phi>)"
-  using assms
+    using assms
 proof (induction \<phi> arbitrary: s t \<rho>)
   case (Atom i p)
   then show ?case
-    using atoms[of s t i] by simp
+    by (simp add: atoms) 
 next
   case (Not \<phi>)
-  then show ?case by auto
+  have False using Not.prems(3) by (rule pos_NotE)
+  then show ?case by simp
 next
-  case (And \<phi> \<psi>)
-  then show ?case by auto
-next
-case (Var X)
-  have "(s \<in> \<rho> X) \<longleftrightarrow> (t \<in> lift_env \<rho> X)"
-    proof
-      assume "s \<in> \<rho> X"
-      with Var.prems(1) show "t \<in> lift_env \<rho> X"
-        by (auto simp: lift_env_def)
-    next
-      assume "t \<in> lift_env \<rho> X"
-      then obtain s' where "s' \<in> \<rho> X" "(s',t) \<in> R"
-        by (auto simp: lift_env_def)
-      with Var.prems(1) have "(s,s') \<in> R_src"
-        by (auto simp: R_src_def)
-      moreover have "R_closed (\<rho> X)"
-        using Var.prems(2) by (auto simp: env_R_closed_def)
-      ultimately show "s \<in> \<rho> X"
-        using \<open>s' \<in> \<rho> X\<close> by (auto simp: R_closed_def)
-    qed
-  then show ?case by simp 
+  case (And \<phi>1 \<phi>2)
+  have pos1: "pos X \<phi>1" using And.prems(3) by (rule pos_And_inv1)
+  have pos2: "pos X \<phi>2" using And.prems(3) by (rule pos_And_inv2)
+
+  have IH1: "s \<in> eval M \<rho> \<phi>1 \<longleftrightarrow> t \<in> eval N (lift_env \<rho>) \<phi>1"
+    using And.IH(1)[OF And.prems(1) And.prems(2) pos1] .
+
+  have IH2: "s \<in> eval M \<rho> \<phi>2 \<longleftrightarrow> t \<in> eval N (lift_env \<rho>) \<phi>2"
+    using And.IH(2)[OF And.prems(1) And.prems(2) pos2] .
+
+  with IH1 IH2 show ?case by simp
 next
   case (Dia i a \<phi>)
   show ?case 
@@ -311,10 +375,13 @@ next
                   and rel:   "(s(i := u i), t(i := t')) \<in> R"
       by (metis (no_types, lifting) iso_tuple_UNIV_I mem_Collect_eq
           move_i_def)
+
+    have pos\<phi>: "pos X \<phi>" using Dia.prems(3) by (rule pos_Dia_inv)
     
-    from Dia.IH
-    have "s(i := u i) \<in> eval M \<rho> \<phi> \<longleftrightarrow> t(i := t') \<in> eval N (lift_env \<rho>) \<phi>"
-      using Dia.prems(2) rel by presburger 
+    have IH_inst:
+      "s(i := u i) \<in> eval M \<rho> \<phi> \<longleftrightarrow> t(i := t') \<in> eval N (lift_env \<rho>) \<phi>"
+      using Dia.IH[OF rel Dia.prems(2) pos\<phi>] .
+
     from umv have u_eq: "u = s(i := u i)"
       using move_i_def by fastforce
     with u\<phi> have "s(i := u i) \<in> eval M \<rho> \<phi>"
@@ -341,9 +408,12 @@ next
                 and rel2:  "(s(i := s_i), t(i := v i)) \<in> R"
       by blast
 
-    from Dia.IH
-    have "s(i := s_i) \<in> eval M \<rho> \<phi> \<longleftrightarrow> t(i := v i) \<in> eval N (lift_env \<rho>) \<phi>"
-      using Dia.prems(2) rel2 by blast 
+    have pos\<phi>: "pos X \<phi>" using Dia.prems(3) by (rule pos_Dia_inv)
+
+    have IH_inst':
+      "s(i := s_i) \<in> eval M \<rho> \<phi> \<longleftrightarrow> t(i := v i) \<in> eval N (lift_env \<rho>) \<phi>"
+      using Dia.IH[OF rel2 Dia.prems(2) pos\<phi>] .
+
     then have "s(i := s_i) \<in> eval M \<rho> \<phi>"
       using v\<phi> vshape
       by (metis (no_types, lifting) ext fun_upd_other fun_upd_same) 
@@ -356,15 +426,197 @@ next
   case (Perm \<pi> \<phi>)
   (* R is closed under permuting coordinates *)
   have rel\<pi>: "(perm_tup \<pi> s, perm_tup \<pi> t) \<in> R"
-    using Perm.prems(1) by (rule perm) 
-  from Perm.IH
+    using Perm.prems(1) by (rule perm)
+
+  (* Positivity passes through Perm, needed to apply the IH on \<phi> *)
+  have pos\<phi>: "pos X \<phi>"
+    using Perm.prems(3) by (rule pos_Perm_inv)
+
+  (* Apply the IH at the permuted pair *)
   have "perm_tup \<pi> s \<in> eval M \<rho> \<phi> \<longleftrightarrow> perm_tup \<pi> t \<in> eval N (lift_env \<rho>) \<phi>"
-    using Perm.prems(2) rel\<pi> by blast 
+    using Perm.IH[OF rel\<pi> Perm.prems(2) pos\<phi>] .
+
   then show ?case by simp
-next 
+next
+  case (Var x)
+  have "s \<in> \<rho> x \<longleftrightarrow> t \<in> lift_env \<rho> x"
+  proof (rule iffI)
+    assume hs: "s \<in> \<rho> x"
+    from Var.prems(1) have "(s,t) \<in> R" .
+    with hs show "t \<in> lift_env \<rho> x"
+      by (auto simp: lift_env_def)
+  next
+    assume ht: "t \<in> lift_env \<rho> x"
+    then obtain s' where s'in: "s' \<in> \<rho> x" and s'R: "(s',t) \<in> R"
+      by (auto simp: lift_env_def)
+
+    from Var.prems(1) have st: "(s,t) \<in> R" .
+
+    (* turn the two R-edges with common right node t into a pair in R_src *)
+    have "(s,s') \<in> R_src"
+      using st s'R by (auto simp: R_src_def)
+
+    (* use that \<rho> is R-closed componentwise *)
+    have "R_closed (\<rho> x)"
+      using Var.prems(2) by (auto simp: env_R_closed_def)
+
+    from this and \<open>(s,s') \<in> R_src\<close> and s'in
+    show "s \<in> \<rho> x"
+      by (auto simp: R_closed_def)
+  qed
+  then show ?case by simp
+next
   case (Mu X \<phi>)
-  then show ?case sorry
-next 
+  define F  where "F  S = eval M (\<rho>(X := S))  \<phi>" for S
+  define G  where "G  T = eval N ((lift_env \<rho>)(X := T)) \<phi>" for T
+
+  have mono_F: "mono F" 
+  proof (rule monoI)
+    fix S T :: "(('\<iota>,'s) tup) set"
+    assume "S \<subseteq> T"
+    then have "\<rho>(Y := S) \<sqsubseteq> \<rho>(Y := T)" for Y
+      by (simp add: env_le_update) 
+    then have "eval M (\<rho>(Y := S)) \<phi> \<subseteq> eval M (\<rho>(Y := T)) \<phi>" for Y
+      by (smt (verit, best) Mu.prems(3) eval_mono_env pfml.distinct(11,33,47,51,55)
+          pfml.inject(7) pfml.simps(50) pos.cases)
+    then show "F S \<subseteq> F T" unfolding F_def by simp
+  qed
+
+  have mono_G: "mono G" 
+  proof (rule monoI)
+    fix T U :: "(('\<iota>,'t) tup) set"
+    assume "T \<subseteq> U"
+    hence "((lift_env \<rho>)(X := T)) \<sqsubseteq> ((lift_env \<rho>)(X := U))"
+      by (simp add: env_le_update)
+    hence "eval N ((lift_env \<rho>)(X := T)) \<phi> \<subseteq> eval N ((lift_env \<rho>)(X := U)) \<phi>"
+      using Mu.prems(3)
+      by (smt (verit) eval_mono_env pfml.distinct(11,33,41,47,51,55) pfml.inject(7)
+          pos.cases) (* pos X \<phi> *) 
+    then show "G T \<subseteq> G U" unfolding G_def by simp
+  qed
+
+  (* If S is R-closed then both updated envs are R-closed. *)
+  have env_closed_upd:
+    "R_closed S \<Longrightarrow> env_R_closed (\<rho>(X := S))" for S
+    using Mu.prems(2)
+    by (auto simp: env_R_closed_def R_closed_def)
+
+  (* IH instantiated on the body, with an updated env and the lifted env on N. *)
+  have IH_upd:
+    "\<lbrakk> (u,v)\<in>R; R_closed S \<rbrakk> \<Longrightarrow>
+       (u \<in> eval M (\<rho>(X := S)) \<phi>) \<longleftrightarrow> (v \<in> eval N (lift_env (\<rho>(X := S))) \<phi>)"
+    for u v S
+    using Mu.IH[of u v "\<rho>(X := S)"] env_closed_upd Mu.prems(3)
+    by (smt (verit, ccfv_threshold) pfml.distinct(34) pfml.inject(7)
+        pfml.simps(20,50,56,60,64) pos.cases)
+
+  (* Rewrite the N-side env update into the “G (lift_set S)” shape. *)
+  have IH_bridge:
+    "\<lbrakk> (u,v)\<in>R; R_closed S \<rbrakk> \<Longrightarrow>
+       (u \<in> F S) \<longleftrightarrow> (v \<in> G (lift_set S))"
+    for u v S
+    by (simp add: IH_upd F_def G_def lift_env_update)
+
+  (* Every approximant on the M-side is R-closed (by IH on \<phi>). *)
+  have appr_closed: "R_closed (appr F n)" for n 
+  proof (induction n)
+    case 0 show ?case by (simp add: R_closed_def)   (* {} is R-closed *)
+  next
+    case (Suc n)
+    have "env_R_closed (\<rho>(X := appr F n))"
+      using env_closed_upd Suc.IH .
+    (* Use the body-preservation (Mu.IH) to transport membership across R,
+       which gives R_closed of F (appr n) = appr (Suc n). *)
+    show ?case
+    proof (unfold R_closed_def, intro allI impI)
+      fix u v assume "(u,v) \<in> R_src"
+      then obtain w where uw: "(u,w)\<in>R" and vw: "(v,w)\<in>R"
+        by (auto simp: R_src_def)
+      have "(u \<in> F (appr F n)) \<longleftrightarrow> (w \<in> G (lift_set (appr F n)))"
+        using IH_bridge[OF uw Suc.IH] .
+      moreover have "(v \<in> F (appr F n)) \<longleftrightarrow> (w \<in> G (lift_set (appr F n)))"
+        using IH_bridge[OF vw Suc.IH] .
+      ultimately show "u \<in> appr F (Suc n) \<longleftrightarrow> v \<in> appr F (Suc n)"
+        by simp   
+    qed
+  qed
+
+(* Synchronization: approximants correspond pointwise along R. *) 
+  have appr_sync: "(u,v) \<in> R \<Longrightarrow> (u \<in> appr F n \<longleftrightarrow> v \<in> appr' G n)" for u v n 
+  proof (induction n arbitrary: u v) 
+    case 0 
+    then show ?case by simp 
+  next 
+    case (Suc n u v) 
+    from Suc.prems have uv: "(u,v) \<in> R" . 
+    have IHn: "(w,z)\<in>R \<Longrightarrow> (w \<in> appr F n \<longleftrightarrow> z \<in> appr' G n)" for w z 
+      using Suc.IH by blast 
+    have "u \<in> appr F (Suc n) \<longleftrightarrow> u \<in> F (appr F n)" 
+      by simp also have "... \<longleftrightarrow> v \<in> G (appr' G n)" 
+    proof - 
+      have PRES_\<phi>: "u \<in> eval M (\<rho>(X := appr F n)) \<phi> \<longleftrightarrow> v \<in> eval N ((lift_env \<rho>)(X := appr' G n)) \<phi>" 
+        sorry 
+      then show ?thesis 
+        unfolding F_def G_def by blast 
+    qed 
+    also have "... \<longleftrightarrow> v \<in> appr' G (Suc n)" 
+      by simp 
+    finally show ?case . 
+  qed
+  have appr_pre_fix: "F (\<Union>n. appr F n) \<subseteq> (\<Union>n. appr F n)" 
+  proof 
+    fix u assume "u \<in> F (\<Union>n. appr F n)" 
+    then obtain n where "u \<in> F (appr F n)" 
+      using mono_F sorry 
+    thus "u \<in> (\<Union>n. appr F n)" 
+      by (metis UNIV_I UN_I appr_Suc) 
+  qed 
+  have appr_le_lfp: "appr F n \<subseteq> lfp F" for n 
+    apply (induction n) 
+     apply simp 
+    by (metis lfp_fixpoint mono_F monotoneD prod_bisim.appr_Suc prod_bisim_axioms) 
+  have lfpF_eq: "lfp F = (\<Union>n. appr F n)" 
+  proof (rule antisym) 
+    show "lfp F \<subseteq> (\<Union>n. appr F n)" 
+    proof (rule lfp_lowerbound) 
+      show "F (\<Union>n. appr F n) \<subseteq> (\<Union>n. appr F n)" 
+        by (rule appr_pre_fix) 
+    qed 
+    show "(\<Union>n. appr F n) \<subseteq> lfp F" 
+      using appr_le_lfp by blast 
+  qed 
+
+  (* The same for G / appr' *) 
+  have appr'_pre_fix: "G (\<Union>n. appr' G n) \<subseteq> (\<Union>n. appr' G n)" 
+  proof fix v assume "v \<in> G (\<Union>n. appr' G n)" 
+    then obtain n where "v \<in> G (appr' G n)" 
+      using mono_G sorry 
+    thus "v \<in> (\<Union>n. appr' G n)" 
+      by (metis UNIV_I UN_iff appr'_Suc) 
+  qed 
+  have appr'_le_lfp: "appr' G n \<subseteq> lfp G" for n 
+    apply (induction n) 
+     apply simp 
+    by (metis lfp_fixpoint mono_G monotoneD prod_bisim.appr'_Suc prod_bisim_axioms) 
+  
+  have lfpG_eq: "lfp G = (\<Union>n. appr' G n)" 
+  proof (rule antisym) 
+    show "lfp G \<subseteq> (\<Union>n. appr' G n)" 
+      by (simp add: appr'_pre_fix lfp_lowerbound) 
+    show "(\<Union>n. appr' G n) \<subseteq> lfp G" 
+      using appr'_le_lfp by blast 
+  qed
+
+  have "s \<in> lfp F \<longleftrightarrow> t \<in> lfp G"
+  proof -
+    have "(s \<in> (\<Union>n. appr F n)) \<longleftrightarrow> (t \<in> (\<Union>n. appr' G n))"
+      using appr_sync[OF Mu.prems(1)] by blast
+    then show ?thesis by (simp add: lfpF_eq lfpG_eq)
+  qed
+
+  then show ?case
+    unfolding F_def G_def by simp 
+next
   case (Nu X \<phi>)
   then show ?case sorry
 qed
